theories/goedel/PRrepresentable.v
@@ -42,14 +42,14 @@ Definition beta (a z : nat) : nat :=
           (cPairPi2 a))).
 
 Definition betaFormula : Formula :=
-exH 3
+existH 3
   (v_ 3 < S_ (v_ 2) /\
-   exH 4
+   existH 4
      (v_ 4 < S_ (v_ 2) /\
       (v_ 3 + v_ 4) * S_ (v_ 3 + v_ 4) + natToTerm 2 * v_ 3 =
       natToTerm 2 * v_ 2 /\
       v_ 0 < S_ (v_ 3 * S_ (v_ 1)) /\
-      exH 5 (v_ 5 < S_ (v_ 4) /\ v_ 0 +  
+      existH 5 (v_ 5 < S_ (v_ 4) /\ v_ 0 +  
                                    v_ 5 * S_ (v_ 3 * S_ (v_ 1)) = v_ 4)))%nn.
  
 Lemma betaRepresentable : Representable 2 beta betaFormula.
